ONGOING: PCF and variability

src/cia.lean
@@ -8,8 +8,18 @@ namespace CIA
 
 constant SysElCount: ℕ
 constant GSNElCount: ℕ
+
+@[derive fintype, derive decidable_eq]
 def SysEl: Type := fin SysElCount
+
+@[derive fintype]
+def SySEls := set SysEl 
+
+@[derive fintype, derive decidable_eq]
 def GSNEl: Type := fin GSNElCount
+
+@[derive fintype]
+def GSNEls := set GSNEl
 
 --section
 
@@ -23,55 +33,68 @@ inductive Annotation : Type
 --variables (GSNEl : Type) [finGSNEl: fintype GSNEl] [deqGSNEl: decidable_eq GSNEl]
 
 @[reducible]
-def Sys : Type := finset SysEl
+def Sys : Type := set SysEl --finset SysEl
 
 --@[reducible, simp]
 --instance SysEl_has_union: has_union (finset SysEl) := @finset.has_union SysEl deqSysEl
 
 @[reducible]
-def GSN : Type := finset GSNEl
+def GSN : Type := set GSNEl --finset GSNEl
 
 @[reducible]
-def TraceRel : Type := finset (SysEl × GSNEl)
+def TraceRel : Type := set (SysEl × GSNEl) --finset (SysEl × GSNEl)
 
-variable sliceSys   (s : Sys)  (es : finset SysEl) : Sys
-variable sliceGSN_V (ac : GSN) (es : finset GSNEl) : GSN
-variable sliceGSN_R (ac : GSN) (es : finset GSNEl) : GSN
+variable sliceSys   (s : Sys)  (es : set SysEl) : Sys
+variable sliceGSN_V (ac : GSN) (es : set GSNEl) : GSN
+variable sliceGSN_R (ac : GSN) (es : set GSNEl) : GSN
 
 structure Delta :=
-(add : finset SysEl) (delete : finset SysEl) (modify : finset SysEl)
+(add : set SysEl) (delete : set SysEl) (modify : set SysEl)
 
-def allElements (d: Delta) : finset SysEl :=
+def allElements (d: Delta) : set SysEl :=
      (d.add ∪ d.delete ∪ d.modify)
 
-def restrict (t : TraceRel) (d : Delta) : TraceRel :=
-    finset.filter (λx, x.1 ∈ allElements d) t
+def restrict (t : TraceRel) (d : Delta) : TraceRel := 
+    {x:(SysEl × GSNEl) | x ∈ t ∧ x.1 ∈ allElements d }
     
-def trace (t : TraceRel) (es : finset SysEl) : finset GSNEl :=
-    finset.image (λx:(SysEl × GSNEl), x.2) 
-        (finset.filter (λ e:(SysEl × GSNEl), e.1 ∈ es) t)
+def trace (t : TraceRel) (es : set SysEl) : set GSNEl :=
+    set.image (λx:(SysEl × GSNEl), x.2) 
+        {e: (SysEl × GSNEl) | e ∈ t ∧ e.1 ∈ es }
+        --(set.filter (λ e:(SysEl × GSNEl), e.1 ∈ es) t)
 
-def createAnnotation'   (recheck : finset GSNEl)
-                        (revise : finset GSNEl) 
-                        (el: GSNEl) 
+/-
+def createAnnotation'   (recheck:   set GSNEl)
+                        (revise:    set GSNEl) 
+                        (el:        GSNEl) 
                         : Annotation :=
-@dite 
-    Annotation 
-    (el ∈ recheck) 
-    (finset.decidable_mem el recheck) 
-    (λ_, Annotation.Recheck)
+if 
+    --Annotation 
+    (el ∈ recheck) then
+    --(set.decidable_mem el recheck) 
+    (λ_, Annotation.Recheck) else
     (λ_, @dite 
         Annotation
         (el ∈ revise) 
-        (finset.decidable_mem el revise)
+        (set.decidable_mem_of_fintype revise el)
         (λ_,  Annotation.Revise) 
-        (λ_, Annotation.Reuse))
+        (λ_, Annotation.Reuse)) .
 
 def createAnnotation    (g : GSN) 
-                        (recheck : finset GSNEl)
-                        (revise : finset GSNEl) 
-                        : finset (GSNEl × Annotation) :=
-    finset.image (λx, (x, createAnnotation' recheck revise x)) g
+                        (recheck : set GSNEl)
+                        (revise : set GSNEl) 
+                        : set (GSNEl × Annotation) :=
+    set.image (λx, (x, createAnnotation' recheck revise x)) g
+-/
+
+def createAnnotation    (g : GSN) 
+                        (recheck : set GSNEl)
+                        (revise : set GSNEl)
+                    : set (GSNEl × Annotation) :=
+    let ch := image (λ e, (e, Annotation.Recheck)) recheck,
+        rv := image (λ e, (e, Annotation.Revise)) revise,
+        ru := image (λ e, (e, Annotation.Reuse)) 
+                    (g \ (recheck ∪ revise))
+    in  ch ∪ rv ∪ ru
 
 open Delta
 
@@ -80,7 +103,7 @@ def GSN_IA  (S  : Sys)
             (A  : GSN)
             (R  : TraceRel)
             (D  : Delta)
-            : finset (GSNEl × Annotation) :=
+            : set (GSNEl × Annotation) :=
     let R'          := restrict R D,
         C1dm        := sliceSys S (D.delete ∪ D.modify),
         C1am        := sliceSys S' (D.add ∪ D.modify),
@@ -89,6 +112,6 @@ def GSN_IA  (S  : Sys)
         C3Recheck1  := sliceGSN_V A C2Revise,
         C3Recheck2  := sliceGSN_R A (C2Recheck ∪ C3Recheck1)
     in  createAnnotation A C3Recheck2 C2Revise
-    
+
 end CIA
 
