src/liftedSet.lean
@@ -11,61 +11,128 @@ def PC := Prop
 structure Var (α : Type) := 
     (v : α) (pc : PC) 
 
-def set' (α : Type) [fintype α] [decidable_eq α]: Type := α → PC
+def set' (α : Type) /-[fintype α] [decidable_eq α]-/: Type := α → PC
 
 @[class]
 structure has_index (α : Type) {β : Type} :=
 (index_ : α → PC → β )
 
-def index {α:Type} [fintype α] [decidable_eq α]
-    (s : set' α) (pc : PC) : set α := (and pc) ∘ s
+--def to_finset {α: Type} [f: fintype α] (s: set α): finset α :=
+--set.finite.to_finset --to_finset 
+--set.finite.coe_to_finset (set.finite.of_fintype s)
+    --set.univ_finite_iff_nonempty_fintype f f.elems ∩ s 
+    --@set.to_finset α s (set.finite.fintype (@set.fintype α f)) -- ↥s)
 
-protected def mem {α:Type} [fintype α] [decidable_eq α] 
-    (x : Var α) (s : set' α) : Prop := x.2 → (s x.1)
+#print finset.finite_to_set
+#print fintype.of_finset
+#print finset.fintype_coe_sort
+#print set.finite.coe_sort_to_finset
+#print finset.finite_to_set_to_finset
 
-instance {α:Type} [fintype α] [decidable_eq α]: 
-    has_mem (Var α) (set' α) := ⟨liftedSet.mem⟩
+--@[simp]
+--noncomputable
+--def to_finite {α: Type} [f: fintype α] (s: set α) : finset α :=
+    --set.finite.coe_to_finset 
+--    (set.finite.of_fintype s).to_finset
 
-protected def subset {α:Type} [fintype α] [decidable_eq α]
+--noncomputable
+def index {α:Type} --[f: fintype α] [decidable_eq α]
+    (s : set' α) (pc : PC) : set α := ((and pc) ∘ s)
+        --@set.to_finset α ((and pc) ∘ s) (fintype.of_finset f) --(@finset.fintype α f)
+
+--protected def mem {α:Type} [fintype α] [decidable_eq α] 
+--    (x : Var α) (s : set' α) : Prop := x.2 → (s x.1)
+
+--instance {α:Type} [fintype α] [decidable_eq α]: 
+--    has_mem (Var α) (set' α) := ⟨liftedSet.mem⟩
+
+--@[simp]
+instance liftedSet_has_mem {α:Type}: --[fintype α] [decidable_eq α]: 
+    has_mem α (set' α) := ⟨λx s, s x⟩
+
+protected def subset {α:Type} --[fintype α] [decidable_eq α]
     (s₁ s₂ : set' α) : Prop := ∀ a, a ∈ s₁ → a ∈ s₂
 
-instance {α:Type} [fintype α] [decidable_eq α]: 
+instance {α:Type}:-- [fintype α] [decidable_eq α]: 
     has_subset (set' α) := ⟨ liftedSet.subset ⟩
 
-protected def sub {α : Type} [fintype α] [decidable_eq α] 
+protected def sub {α : Type}-- [fintype α] [decidable_eq α] 
     (s₁ s₂ : set' α) : set' α := λ (a : α), s₁ a ∧ ¬ (s₂ a)
 
-instance {α:Type} [fintype α] [decidable_eq α]: 
+instance {α:Type}:-- [fintype α] [decidable_eq α]: 
     has_sub (set' α) := ⟨ liftedSet.sub ⟩
 
-protected def union {α:Type} [fintype α] [decidable_eq α]
+protected def union {α:Type}-- [fintype α] [decidable_eq α]
     (s₁ s₂ : set' α) : set' α := λ x, (s₁ x) ∨ (s₂ x)
 
-instance {α:Type} [fintype α] [decidable_eq α]: 
+instance {α:Type}:-- [fintype α] [decidable_eq α]: 
     has_union (set' α) := ⟨liftedSet.union⟩
 
-protected def diff {α:Type} [fintype α] [decidable_eq α] 
+protected def diff {α:Type}-- [fintype α] [decidable_eq α] 
     (s₁ s₂ : set' α) : set' α := λ x, (s₁ x) ∧ ¬(s₂ x)
 
-instance {α: Type } [fintype α] [decidable_eq α]: 
+instance {α: Type }:-- [fintype α] [decidable_eq α]: 
     has_sdiff (set' α) := ⟨liftedSet.diff⟩
-
-def image_ {α:Type} {β:Type} [fintype α] [decidable_eq α]
-    (f : α → β) (s : set' α) : set (β × PC) :=
-        {y: β×PC | ∃ x, (y.1 = f x) ∧ (s x = y.2)}
-
---finset.filter 
- 
---def image {α:Type} {β:Type} (f : α → β) (s : set' α) : set' β :=
---{(y,pc) | ∃ x, x ∈ α ∧ (y = f x) ∧ (s y = pc)}  
---λ x, (∀ y, f y = x ∧ s y)  
 
 infix `|`:90 := index
 
-variables [fintype α] [decidable_eq α] [fintype β] [decidable_eq β] [fintype γ] [decidable_eq γ]
+--def image_ {α:Type} {β:Type} --[fintype α] [decidable_eq α]
+--    (f : α → β) (s : set' α) : set (β × PC) :=
+--        {y: β×PC | ∃ x, (y.1 = f x) ∧ (s x = y.2)}
+
+--finset.filter 
+ 
+#print set.image
+#print finset.subtype.fintype
+
+instance or_is_commutative: is_commutative PC or := ⟨ λ a b, propext (or_comm a b) ⟩
+instance or_is_associative: is_associative PC or := ⟨ λ a b _, propext (or_assoc a b) ⟩
+
+def image {α:Type} [fintype α] {β:Type} 
+(f : α → β) (s : set' α) : set' β :=
+λ x, let r := {z | f(z) = x} in 
+    finset.fold or true s (set.finite.to_finset (set.finite.of_fintype r))   
+
+lemma index_image {α: Type} [fintype α] {β: Type} (f: α→β) (s: set' α) (pc: PC):
+    (image f s) | pc = set.image f (s|pc) :=
+begin 
+    --rw set.image, 
+    rw image, unfold set.finite.to_finset, rw index, rw function.comp, rw set_of, apply funext, intros, 
+    simp, split, 
+    {intros h, apply and.elim h, intros h₁ h₂, let y:α,   } 
+end
+
+lemma index_union {α: Type} (x: α) (pc: PC) (s₁ s₂: set' α): 
+    (x ∈ s₁|pc ∨ x ∈ s₂|pc) = (x ∈ (s₁ ∪ s₂)|pc) :=
+begin
+    intros, repeat {rw index}, repeat {rw function.comp}, 
+    repeat {rw set.mem_def}, simp, rw← and_or_distrib_left, refl 
+end
+
+lemma index_mem {α: Type} (x:α) (pc: PC) (s: set' α):
+    (x ∈ s|pc) = ((x ∈ s) ∧ pc) :=
+begin
+    unfold index, unfold function.comp, unfold has_mem.mem,
+    unfold set.mem, rw and_comm
+end
+
+-- filter
+def filter {α: Type} (p: α → Prop) (s: set' α): 
+    set' α := λx, p x ∧ s x
+
+/-
+theorem filter_correct {α:Type} [fintype α] [decidable_eq α] (p: α → Prop) (s: set' α) (pc: PC) [decidable_pred p]:
+    filter p s | pc = finset.filter p (s | pc) :=
+begin
+    unfold index, repeat {unfold function.comp}, unfold filter,
+    simp, rw finset.finite_to_set_to_finset, rw set.to_finset, 
+end 
+-/
+
+variables --[fintype α] [decidable_eq α] [fintype β] [decidable_eq β] [fintype γ] [decidable_eq γ]
     (f₁  : set  α → set  β) (f₂  : set  β  → set  γ)
     (f₁' : set' α → set' β) (f₂' : set' β  → set' γ)
-    
+
 theorem fun_comp_correct :
     (∀ a ρ, (f₁ (a | ρ) = (f₁' a) | ρ)) →
     (∀ b ρ, (f₂ (b | ρ) = (f₂' b) | ρ)) →
