src/PCF.lean
@@ -1,0 +1,181 @@
+import data.finset
+import tactic.induction
+
+namespace PCF
+
+-- vname: variable name
+def vname := string
+
+@[derive [decidable_eq]]
+inductive τ 
+| Nat : τ
+| Bool : τ
+| Arrow : τ → τ → τ
+
+def to_string_τ : τ → string
+| τ.Nat           := "ℕ"
+| τ.Bool          := "Bool"
+| (τ.Arrow t₀ t₁) := (to_string_τ t₀) ++ " → " ++ (to_string_τ t₁)
+
+instance : has_to_string τ := ⟨to_string_τ⟩
+instance : has_repr τ := ⟨to_string_τ⟩
+
+inductive expr
+| Zero : expr
+| succ : expr → expr
+--| pred : expr → expr
+| True : expr
+| False : expr
+| zero : expr → expr
+| Var : vname → expr
+| ITE : expr → expr → expr → expr
+| LAM : vname → τ → expr → expr
+| APP : expr → expr → expr
+| FIX : vname → τ → expr → expr
+
+-- fv: free variables in expressions
+def fv : expr → finset vname
+| expr.Zero         := ∅ 
+| (expr.succ e)     := fv e
+--| (expr.pred e)     := fv e
+| expr.True         := ∅ 
+| expr.False        := ∅
+| (expr.zero e)     := fv e
+| (expr.Var v)      := {v}
+| (expr.ITE c t e)  := (fv c) ∪ (fv t) ∪ (fv e)
+| (expr.LAM v t b)  := (fv b) \ {v}
+| (expr.APP e₀ e₁)  := (fv e₀) ∪ (fv e₁)
+| (expr.FIX v t b)  := (fv b) \ {v} 
+
+-- substitution
+def sub (s: expr) (v: vname) : expr → expr
+| expr.Zero         := expr.Zero
+| (expr.succ e')    := expr.succ (sub e')
+--| (expr.pred e')    := expr.pred (sub e')
+| expr.True         := expr.True
+| expr.False        := expr.True
+| (expr.zero e')    := expr.zero (sub e')
+| (expr.Var v')     := if v = v' then s else expr.Var v'
+| (expr.ITE c t e') := expr.ITE (sub c) (sub t) (sub e')
+| (expr.LAM v' t b) := if v = v' then expr.LAM v' t b else expr.LAM v' t (sub b)
+| (expr.APP e₀ e₁)  := expr.APP (sub e₀) (sub e₁)
+| (expr.FIX v' t b) := if v = v' then expr.FIX v' t b else expr.FIX v' t (sub b)
+
+-- type environment
+def env : Type := vname → option τ
+def emptyEnv : env := λ x, none
+def addType (Γ: env) (v: vname) (t: τ) : env := 
+λ x, if (x = v) then (some t) else (Γ x)
+
+-- typing function
+def typing : env → expr → option τ
+| _ expr.Zero         := τ.Nat
+| Γ (expr.succ e)     := if typing Γ e = some τ.Nat then some τ.Nat else none 
+--| Γ (expr.pred e)     := if typing Γ e = some τ.Nat then some τ.Nat else none
+| _ expr.True         := τ.Bool
+| _ expr.False        := τ.Bool
+| Γ (expr.zero e)     := if typing Γ e = some τ.Nat then some τ.Bool else none
+| Γ (expr.Var v)      := Γ v
+| Γ (expr.ITE c t e)  := if (typing Γ c = some τ.Bool) && (typing Γ t = typing Γ e) then typing Γ t else none
+| Γ (expr.LAM v t b)  := let tb := (typing (addType Γ v t)) b in
+                         match tb with
+                         | none     := none
+                         | some t'  := τ.Arrow t t'
+                         end
+| Γ (expr.APP e₀ e₁)  := let t₀ := typing Γ e₀,
+                             t₁ := typing Γ e₁ in
+                         match t₀, t₁ with
+                         | some (τ.Arrow t' t''), some t''' := if (t' = t''') then (some t'') else none
+                         | _, _ := none
+                         end
+| Γ (expr.FIX v t b)  := let tb := (typing (addType Γ v t)) b in
+                         match tb with
+                         | some t' := if t = t' then some t else none
+                         | _ := none
+                         end
+
+namespace operational
+-- call-by-value operational semantics of PCF
+
+-- values (normal forms)
+inductive val : expr → Prop
+| zero : val expr.Zero
+| true : val expr.True
+| false : val expr.False
+| succ {e} (h: val e) : val (expr.succ e)
+--| pred {e} (h: val e) : val (expr.pred e)
+| lam {v} {t} {e} : val (expr.LAM v t e)
+
+inductive big_step : expr → expr → Prop
+-- reduction rules
+--| v {e} (h: val e) : big_step e e
+| succ {e e'} (h: big_step e e'): big_step (expr.succ e) (expr.succ e')
+--| pred_z: big_step (expr.pred expr.Zero) expr.Zero
+--| pred {e e'} (h: big_step e e') : big_step (expr.pred e) e'
+| zero_t {e} (h: big_step e expr.Zero) : big_step (expr.zero e) (expr.True)
+| zero_f {e e'} (h: big_step e (expr.succ e')) : big_step (expr.zero e) (expr.False)
+--| if_ {c t f c'} (hc: big_step c c'): big_step (expr.ITE c t f) (expr.ITE c' t f)
+| if_t {c t t' e} (hc: big_step c expr.True) (ht : big_step t t'): big_step (expr.ITE c t e) t'
+| if_f {c t e e'} (hc: big_step c expr.False) (ht : big_step e e'): big_step (expr.ITE c t e) e'
+| app_1 {e₀ e₀' e₁} (h: big_step e₀ e₀'): big_step (expr.APP e₀ e₁) (expr.APP e₀' e₁)
+| app_2 {e₀ e₁ e₁'} (h₀: val e₀) (h₁: big_step e₁ e₁'): big_step (expr.APP e₀ e₁) (expr.APP e₀ e₁')
+| app_lam {x t e e₀} (h₀: val e₀): big_step (expr.APP (expr.LAM x t e) e₀) (sub e₀ x e)
+| fix {x t b} : big_step (expr.FIX x t b) (sub (expr.FIX x t b) x b)
+
+infix ` ⟹ ` : 110 := big_step
+
+theorem big_step_deterministic {e₀ e₁ e₂} 
+  (h₀: e₀ ⟹ e₁) (h₁: e₀ ⟹ e₂) : 
+  e₁ = e₂ :=
+begin
+  induction' h₀, 
+    case succ {
+      cases h₁, 
+      simp, 
+      apply ih, 
+      assumption },
+    case zero_t {
+      cases h₁, 
+      refl,
+      have h₂ := ih h₁_h, cases h₂},
+    case zero_f: e₃ e₄ {
+      cases h₁,
+      have h₂ := ih h₁_h, cases h₂,
+      refl },
+    case if_t: e₃ e₄ e₅ e₆ h₂ h₃ h₄ h₅ {
+      apply h₅, cases h₁, assumption,
+      have h₇ := h₄ h₁_hc, cases h₇ },
+    case if_f: e₃ e₄ e₅ e₆ h₂ h₃ h₄ h₅ {
+      apply h₅, cases h₁,
+      have h₇ := h₄ h₁_hc, cases h₇,
+      assumption },
+    case app_1 : e₃ e₄ e₅ {
+      cases h₁,
+        simp, apply ih, assumption,
+        rw (@ih e₃), simp, assumption,
+    },
+    -- easy cases
+    repeat {cases h₁, refl},
+    -- succ 
+    rw ih e₁, 
+    cases h₁, rw h₀_ih, refl,
+    -- true
+    cases h₁, refl,
+end
+
+end operational
+
+namespace denotational
+-- denotational semantics of PCF
+def bot {α : Type} : Type := false → α --:= λf, by contradiction
+
+def lifted_T (α : Type) := (@bot α) ⊕ α
+
+def denoteT : τ → Type
+| τ.Nat := lifted_T ℕ
+| τ.Bool := lifted_T bool
+| (τ.Arrow t₀ t₁) := (denoteT t₀) → (denoteT t₁)
+
+end denotational
+
+end PCF
