src/PCF_test.lean
@@ -1,0 +1,49 @@
+import PCF
+
+open PCF
+
+-- example 5.3.2 from Prof. Marcelo Fiore's lecture notes on 
+-- Denotational Semantics 
+def F := expr.Var "F"
+def G := expr.Var "G"
+def x := expr.Var "x"
+def y := expr.Var "y"
+def h := expr.Var "h"
+
+def Γ₀ := emptyEnv
+def Γ₁ := addType Γ₀ "F" (τ.Arrow τ.Nat τ.Nat)
+def Γ₂ := addType Γ₁ "G" (τ.Arrow τ.Nat 
+                          (τ.Arrow τ.Nat 
+                          (τ.Arrow τ.Nat τ.Nat)))
+
+def H := 
+  expr.FIX (expr.LAM "h" (τ.Arrow τ.Nat (τ.Arrow τ.Nat τ.Nat))
+            (expr.LAM "x" τ.Nat
+             (expr.LAM "y" τ.Nat
+              (expr.ITE (expr.zero y)
+                        (expr.APP F x)
+                        (expr.APP (expr.APP (expr.APP G x)
+                                            (expr.pred y))
+                                  (expr.APP (expr.APP h x)
+                                            (expr.pred y))
+                        )
+              )
+             )
+            ) 
+           )
+
+#check H
+#eval typing Γ₂ H
+
+-- example 5.6.1 (p. 45)
+def V := 
+  expr.LAM "x" τ.Nat 
+    (expr.APP (expr.LAM "y" τ.Nat (expr.Var "y"))
+      expr.Zero)
+
+#check V
+#eval typing Γ₀ V
+
+def V' := expr.LAM "x" τ.Nat (expr.Zero)
+#check V'
+#eval typing Γ₀ V'
